gset.fst
@@ -12,6 +12,8 @@ let rec unique_s l =
 
 type s = l:list nat {unique_s l}
 
+let init = []
+
 val filter_uni : f:(nat -> bool)
                -> l:list nat
                -> Lemma (requires (unique_s l))
@@ -48,18 +50,46 @@ let app_op s1 (id, (Add ele)) = if (mem ele s1) then s1 else ele::s1
 #set-options "--query_stats"
 val sim : tr:ae op
         -> s1:s
-        -> Tot (b:bool {b = true <==> (forall e. mem e s1 <==> mem_ele e tr.l)})
+        -> Tot (b:bool {b = true <==> (forall e. mem e s1 <==> mem_ele e tr.l) /\ (tr.l = [] <==> s1 = init)})
 
 #set-options "--z3rlimit 1000000"
 let sim tr s1 = 
   forallb (fun e -> (existsb (fun e1 -> e1 = (get_id e1, (Add e))) tr.l)) s1 &&
   forallb (fun e -> mem (get_ele e) s1) tr.l
 
+val remove_st : ele:nat
+              -> s1:s {mem ele s1}
+              -> Tot (s2:s {forall e. mem e s2 <==> mem e s1 /\ e <> ele})
+let rec remove_st ele s1 =
+  match s1 with
+  |x::xs -> if x = ele then xs else x::remove_st ele xs
+
+val lemma7 : tr:ae op -> s1:s -> tr1:ae op
+           -> Lemma (requires sim tr s1 /\ (forall e. mem e tr1.l <==> mem e tr.l) /\
+                           (forall e e1. mem e tr1.l /\ mem e1 tr1.l /\ get_id e <> get_id e1 /\ tr1.vis e e1 <==>
+                                    mem e tr.l /\ mem e1 tr.l /\ get_id e <> get_id e1 /\ tr.vis e e1))
+                   (ensures (sim tr1 s1))
+                   (decreases %[tr.l;s1;tr1.l])
+
+#set-options "--z3rlimit 10000000"
+let rec lemma7 tr s1 tr1 = 
+  (*)match tr.l, tr1.l with
+  |[], [] -> ()
+  |(id, (Add v))::xs, _ -> 
+        if (mem_ele v xs) then lemma7 (remove_op tr (id, (Add v))) s1 (remove_op tr (id, (Add v)))
+          else lemma7 (remove_op tr (id, (Add v))) (remove_st v s1) (remove_op tr (id, (Add v)))
+             |[], (_, (Add v))::xs -> ()*) ()
+
+val pre_cond_merge1 : l:s -> a:s -> b:s
+                    -> Tot (b1:bool {b1=true <==> (forall e. mem e l ==> mem e a /\ mem e b)})
+let pre_cond_merge1 l a b = 
+  forallb (fun e -> mem e a && mem e b) l
+
 val merge1 : l:s
            -> a:s
            -> b:s
            -> Pure s
-             (requires (forall e. mem e l ==> mem e a /\ mem e b))
+             (requires pre_cond_merge1 l a b)
              (ensures (fun u -> (forall e. mem e u <==> mem e a \/ mem e b)))
              (decreases %[l;a;b])
 
@@ -71,6 +101,7 @@ let rec merge1 l a b =
   |[],x::xs,_ -> if mem x b then (merge1 [] xs b) else x::(merge1 [] xs b)
   |[],[], _ -> b
 
+val pre_cond_merge : ltr:ae op -> l:s -> atr:ae op -> a:s -> btr:ae op -> b:s -> Tot bool
 let pre_cond_merge ltr l atr a btr b = true
 
 val merge : ltr:ae op
@@ -83,7 +114,7 @@ val merge : ltr:ae op
                              (forall e. mem e atr.l ==> not (mem_id (get_id e) btr.l)) /\
                              (forall e. mem e ltr.l ==> not (mem_id (get_id e) btr.l)) /\
                              (sim ltr l /\ sim (union ltr atr) a /\ sim (union ltr btr) b))
-                   (ensures (fun r -> (forall e. mem e r <==> mem e a \/ mem e b)))
+                   (ensures (fun r -> r = merge1 l a b))
 
 #set-options "--z3rlimit 10000000"
 let merge ltr l atr a btr b = 
@@ -122,11 +153,14 @@ val convergence : tr:ae op
 let convergence tr a b = ()
 
 instance _ : mrdt s op = {
+  Library.init = init;
   Library.sim = sim;
   Library.pre_cond_op = pre_cond_op;
   Library.app_op = app_op;
   Library.prop_oper = prop_oper;
   Library.pre_cond_merge = pre_cond_merge;
+  Library.pre_cond_merge1 = pre_cond_merge1;
+  Library.merge1 = merge1;
   Library.merge = merge;
   Library.prop_merge = prop_merge;
   Library.convergence = convergence
