alpha_map.fst
@@ -1,0 +1,714 @@
+module Alpha_map
+open FStar.List.Tot
+
+open Library
+
+type op (alpha_op:eqtype) = (nat (*key*) * alpha_op)
+
+val get_key : #o:eqtype -> op1:(nat * op o) -> Tot (k:nat {exists id op2. op1 = (id, (k, op2))})
+let get_key (id, (k, _)) = k
+
+val get_val : #o:eqtype -> op1:(nat * op o) -> Tot (s:o {exists id k. op1 = (id, (k, s))})
+let get_val (id, (k, s)) = s
+
+val get_key_s : #st:eqtype -> s:(nat * st) -> Tot (s1:nat {(exists c. s = (s1,c))})
+let get_key_s (k, _) = k
+
+val mem_key_s : #st:eqtype 
+              -> ele1:nat
+              -> l:list (nat * st)
+              -> Tot (b:bool {b=true <==> (exists c. mem (ele1,c) l) /\ (exists e. mem e l /\ get_key_s e = ele1)})
+let rec mem_key_s ele1 l =
+  match l with
+  |[] -> false
+  |x::xs -> get_key_s x = ele1 || mem_key_s ele1 xs
+
+val unique_key : #st:eqtype -> list (nat * st) -> bool
+let rec unique_key l =
+  match l with
+  |[] -> true
+  |(ele,_)::xs -> not (mem_key_s ele xs) && unique_key xs
+
+val get_val_s1 : #st:eqtype -> s:(nat * st) -> Tot (c:st {(exists i. s = (i,c))})
+let get_val_s1 (_, c) = c
+
+type s (alpha_st:eqtype) = l:list (nat * alpha_st) {unique_key l}
+
+let init_a = []
+
+val get_val_s : #st:eqtype -> #o:eqtype -> {| mrdt st o |}
+              -> i:nat -> s1:s st -> Tot (c:st {(mem_key_s i s1 ==> mem (i,c) s1 /\ (exists e. mem e s1 /\ e = (i,c))) /\ 
+                                         (not (mem_key_s i s1) ==> c = init #st #o)})
+let rec get_val_s #st #o i s1 =
+  match s1 with
+  |[] -> init #st #o
+  |x::xs -> if get_key_s x = i then get_val_s1 x else get_val_s #st #o i xs
+
+val lemma2 : #st:eqtype -> #o:eqtype -> {|mrdt st o|}
+           -> s1:s st
+           -> Lemma (requires true)
+                   (ensures (forall e. mem e s1 ==> (get_val_s #st #o (get_key_s e) s1 = get_val_s1 #st e)))
+let lemma2 #st #o s1 = admit ()
+
+val mem_op : #o:eqtype -> ele1:op o
+           -> l:list (nat * (op o))
+           -> Tot (b:bool {b=true <==> (exists id. mem (id, ele1) l) })
+let rec mem_op ele2 l =
+  match l with
+  |[] -> false
+  |(_, ele1)::xs -> ele1 = ele2 || mem_op ele2 xs
+
+val mem_key : #o:eqtype -> i:nat -> l:list (nat * op o) -> Tot (b:bool {b=true <==> (exists id op. mem (id, (i, op)) l)})
+let rec mem_key ele2 l =
+  match l with
+  |[] -> false
+  |(_, (ele1, _))::xs -> ele1 = ele2 || mem_key ele2 xs
+
+val filter_uni : #op:eqtype 
+               -> f:((nat * op) -> bool)
+               -> l:list (nat * op) 
+               -> Lemma (requires (unique_id l ))
+                       (ensures (unique_id (filter f l)))
+                       [SMTPat (filter f l)]
+let rec filter_uni f l =
+  match l with
+  |[] -> ()
+  |x::xs -> filter_uni f xs
+
+val project_op : #o:eqtype 
+               -> o1:(nat * (op o))
+               -> Tot (o2:(nat * o) {o2 = (get_id o1, get_val o1)})
+let project_op op =
+  match op with
+  |(id, (k, value)) -> (id, value)
+
+val project1 : #o:eqtype
+             -> i:nat
+             -> l:ae (op o)
+             -> Pure (list (nat * o))
+                    (requires true)
+                    (ensures (fun r -> (forall id. mem_id id r <==> (mem_id id l.l /\ get_key (get_eve id l.l) = i)) /\ 
+                                         unique_id r /\ (forall e. mem e l.l /\ get_key e = i ==> mem (project_op e) r)))
+               (decreases List.Tot.length l.l)
+
+#set-options "--z3rlimit 10000000"
+let rec project1 i l =
+  match l.l with
+  |[] -> []
+  |x::xs -> if (get_key x = i) then (project_op x)::project1 i (A l.vis xs) else (project1 i (A l.vis xs))
+
+val project : #o:eqtype
+            -> i:nat
+            -> l:ae (op o)
+            -> Pure (ae o)
+                   (requires true)
+                   (ensures (fun r -> (forall id. mem_id id r.l <==> (mem_id id l.l /\ get_key (get_eve id l.l) = i)) /\ 
+                                     unique_id r.l /\ (forall e. mem e l.l /\ get_key e = i ==> mem (project_op e) r.l) /\
+                   (forall e e1. (get_id e <> get_id e1 /\ mem (get_id e, (i, get_op e)) l.l /\ 
+             mem (get_id e1, (i, get_op e1)) l.l /\ l.vis (get_id e, (i, get_op e)) (get_id e1, (i, get_op e1))) <==> 
+                   (get_id e <> get_id e1 /\ mem e r.l /\ mem e1 r.l /\ r.vis e e1)) /\ not (mem_key i l.l) <==> r.l = []))
+               (decreases length l.l)
+
+#set-options "--z3rlimit 10000000"
+let project i l =
+    (A (fun o o1 -> (mem (get_id o, (i, get_op o)) l.l && mem (get_id o1, (i, get_op o1)) l.l &&  get_id o <> get_id o1 && l.vis (get_id o, (i, get_op o)) (get_id o1, (i, get_op o1)))) (project1 i l))
+
+val pre_cond_op_a : #st1:eqtype -> #o:eqtype -> {|mrdt st1 o|}
+                  -> s1:s st1 -> op1:(nat * op o)
+                  -> Tot (b:bool {b = true <==> pre_cond_op #st1 #o (get_val_s #st1 #o (get_key op1) s1) (project_op op1)})
+let pre_cond_op_a #st1 #o s1 op = 
+    pre_cond_op #st1 #o (get_val_s #st1 #o (get_key op) s1) (project_op op)
+
+val app_op_a : #st1:eqtype -> #o:eqtype -> {|mrdt st1 o|}
+             -> st:s st1 -> op1:(nat * op o)
+             -> Pure (s st1)
+               (requires pre_cond_op_a #st1 #o st op1)
+               (ensures (fun r -> (forall ch. mem_key_s ch r <==> mem_key_s ch st \/ ch = get_key op1) /\ unique_key r /\
+                               (forall ch. ch <> get_key op1 ==> (get_val_s #st1 #o ch st = get_val_s #st1 #o ch r)) /\
+                             (get_val_s #st1 #o (get_key op1) r = 
+                                  (app_op #st1 #o (get_val_s #st1 #o (get_key op1) st) (project_op op1)))))
+
+#set-options "--z3rlimit 10000000"
+let rec app_op_a #st1 #o st op1 =
+  match st with
+  |[] -> [(get_key op1, (app_op (init #st1 #o) (project_op op1)))]
+  |(ch, x)::xs -> if ch = get_key op1 then (ch, (app_op x (project_op op1)))::xs
+                     else (ch, x)::app_op_a xs op1
+
+val unique_keys : list nat -> Tot bool
+let rec unique_keys l =
+    match l with
+    |[] -> true
+    |x::xs -> not (mem x xs) && unique_keys xs
+
+val get_lst : #st: eqtype -> m:s st -> Pure (list nat)
+                     (requires true)
+                     (ensures (fun r -> (forall i. mem i r <==> mem_key_s i m) /\ unique_keys r))
+let rec get_lst m =
+  match m with
+  |[] -> []
+  |(i,x)::xs -> i::get_lst xs
+
+#set-options "--query_stats"
+val sim_a : #st:eqtype -> #o:eqtype -> {|mrdt st o|}
+          -> tr:ae (op o)
+          -> s1:s st
+          -> Tot (b:bool {(b = true) <==> (forall ch. mem_key_s ch s1 <==> mem_key ch tr.l) /\
+                          (forall ch. mem_key_s ch s1 ==> (sim #st #o) (project ch tr) (get_val_s #st #o ch s1)) /\
+                                     (forall e. mem e tr.l ==> (exists e1. mem e1 s1 /\ get_key e = get_key_s e1))})
+#set-options "--z3rlimit 10000000"
+let sim_a #st #o tr s1 =
+  forallb (fun e -> mem_key (get_key_s e) tr.l) s1 &&
+  forallb (fun e -> mem_key_s (get_key e) s1) tr.l &&
+  forallb (fun e -> (sim #st #o) (project (get_key_s e) tr) (get_val_s #st #o (get_key_s e) s1)) s1 &&
+  forallb (fun e -> (existsb (fun e1 -> get_key e = get_key_s e1) s1)) tr.l
+
+val lemma4 : #st:eqtype -> #o:eqtype -> {|mrdt st o|}
+           -> tr:ae (op o) -> s1:s st
+           -> Lemma (requires sim_a tr s1)
+                   (ensures (forall i. (sim #st #o) (project i tr) (get_val_s #st #o i s1)))
+                    [SMTPat (sim_a tr s1)]
+let lemma4 #st #o tr s1 = admit()
+
+val convergence_a1 : #st:eqtype -> #o:eqtype -> {| mrdt st o |} 
+                   -> tr:ae (op o)
+                   -> a:s st
+                   -> b:s st
+                   -> Lemma (requires (sim_a tr a /\ sim_a tr b))
+                         (ensures (forall e. mem_key_s e a <==> mem_key_s e b))
+let convergence_a1 tr a b = ()
+
+val lem_oper1 : #o:eqtype
+              -> tr:ae (op o)
+              -> op:(nat * (op o))
+              -> Lemma (requires (not (mem_id (get_id op) tr.l)) /\
+                                (forall e. mem e tr.l ==> get_id e < get_id op) /\ get_id op > 0)
+                      (ensures (forall e. mem e (project (get_key op) (append tr op)).l <==> 
+                                     mem e (append (project (get_key op) tr) (project_op op)).l))
+#set-options "--z3rlimit 10000000"
+let lem_oper1 tr op = ()
+
+val lem_oper2 : #o:eqtype
+              -> tr:ae (op o)
+              -> op:(nat * (op o))
+              -> Lemma (requires (not (mem_id (get_id op) tr.l)) /\
+                                (forall e. mem e tr.l ==> get_id e < get_id op) /\ get_id op > 0)
+                      (ensures (forall e e1. mem e (project (get_key op) (append tr op)).l /\
+                        mem e1 (project (get_key op) (append tr op)).l /\ (get_id e <> get_id e1) /\
+                        (project (get_key op) (append tr op)).vis e e1  <==> 
+                        mem e (append (project (get_key op) tr) (project_op op)).l /\
+                    mem e1 (append (project (get_key op) tr) (project_op op)).l /\ get_id e <> get_id e1 /\
+                        (append (project (get_key op) tr) (project_op op)).vis e e1))
+#set-options "--z3rlimit 10000000"
+let lem_oper2 tr op = lem_oper1 tr op
+
+val lem_oper3 : #o:eqtype
+              -> tr:ae (op o)
+              -> op:(nat * (op o))
+              -> Lemma (requires (not (mem_id (get_id op) tr.l)) /\
+                                (forall e. mem e tr.l ==> get_id e < get_id op) /\ get_id op > 0)
+                      (ensures (forall i. i <> (get_key op) ==> (forall e. mem e (project i (append tr op)).l <==> mem e (project i tr).l) /\
+         (forall e e1. mem e (project i (append tr op)).l /\ mem e1 (project i (append tr op)).l /\ get_id e <> get_id e1 /\
+                    (project i (append tr op)).vis e e1 <==> 
+        mem e (project i tr).l /\ mem e1 (project i tr).l /\ get_id e <> get_id e1 /\ (project i tr).vis e e1)))
+#set-options "--z3rlimit 10000000"
+let lem_oper3 tr op = 
+  lem_oper1 tr op;
+  lem_oper2 tr op
+
+val lem_oper : #o:eqtype
+             -> tr:ae (op o)
+             -> op:(nat * (op o))
+             -> Lemma (requires (not (mem_id (get_id op) tr.l)) /\
+                               (forall e. mem e tr.l ==> get_id e < get_id op) /\ get_id op > 0)
+                     (ensures (forall e. mem e (project (get_key op) (append tr op)).l <==> 
+                                    mem e (append (project (get_key op) tr) (project_op op)).l) /\
+               (forall e e1. mem e (project (get_key op) (append tr op)).l /\
+                        mem e1 (project (get_key op) (append tr op)).l /\ (get_id e <> get_id e1) /\
+                        (project (get_key op) (append tr op)).vis e e1  <==> 
+                        mem e (append (project (get_key op) tr) (project_op op)).l /\
+                    mem e1 (append (project (get_key op) tr) (project_op op)).l /\ get_id e <> get_id e1 /\
+                        (append (project (get_key op) tr) (project_op op)).vis e e1) /\
+         (forall i. i <> (get_key op) ==> (forall e. mem e (project i (append tr op)).l <==> mem e (project i tr).l) /\
+         (forall e e1. mem e (project i (append tr op)).l /\ mem e1 (project i (append tr op)).l /\ get_id e <> get_id e1 /\
+                    (project i (append tr op)).vis e e1 <==> 
+        mem e (project i tr).l /\ mem e1 (project i tr).l /\ get_id e <> get_id e1 /\ (project i tr).vis e e1)))
+
+#set-options "--z3rlimit 10000000"
+let lem_oper tr op = 
+  lem_oper1 tr op;
+  lem_oper2 tr op;
+  lem_oper3 tr op
+
+val prop_oper1 : #st1:eqtype -> #o:eqtype -> {|mrdt st1 o|} 
+               -> tr:ae (op o)
+               -> st:s st1
+               -> op1:(nat * (op o)) 
+               -> Lemma (requires (sim_a tr st) /\ (not (mem_id (get_id op1) tr.l)) /\
+                                 (forall e. mem e tr.l ==> get_id e < get_id op1) /\ get_id op1 > 0 /\
+                                 pre_cond_op #st1 #o (get_val_s #st1 #o (get_key op1) st) (project_op op1))
+                       (ensures (forall ch. mem_key_s ch (app_op_a st op1) <==> mem_key ch (append tr op1).l))
+#set-options "--z3rlimit 10000000"
+let prop_oper1 tr st op = lem_oper tr op
+
+val prop_oper2 : #st1:eqtype -> #o:eqtype -> {|mrdt st1 o|} 
+               -> tr:ae (op o)
+               -> st:s st1
+               -> op1:(nat * (op o)) 
+               -> Lemma (requires (sim_a tr st) /\ (not (mem_id (get_id op1) tr.l)) /\
+                                 (forall e. mem e tr.l ==> get_id e < get_id op1) /\ get_id op1 > 0 /\
+                                 pre_cond_op #st1 #o (get_val_s #st1 #o (get_key op1) st) (project_op op1))
+                       (ensures (forall e. mem e (append tr op1).l ==> (exists e1. mem e1 (app_op_a st op1) /\ get_key e = get_key_s e1)))
+
+#set-options "--z3rlimit 10000000"
+let prop_oper2 tr st op = 
+  lem_oper tr op;
+  prop_oper1 tr st op
+
+val lemma1 : #st1:eqtype -> #o:eqtype -> {|mrdt st1 o|}
+         -> tr:ae (op o)
+         -> st:s st1
+         -> op1:(nat * (op o))
+         -> Lemma (requires (sim_a tr st) /\ (not (mem_id (get_id op1) tr.l)) /\
+                           (forall e. mem e tr.l ==> get_id e < get_id op1) /\ get_id op1 > 0 /\
+                           pre_cond_op #st1 #o (get_val_s #st1 #o (get_key op1) st) (project_op op1))
+                 (ensures (forall i. mem_key_s i (app_op_a st op1) /\ i <> get_key op1 ==>
+                   ((forall e. mem e (project i (append tr op1)).l <==> mem e (project i tr).l) /\
+                   (forall e e1. mem e (project i (append tr op1)).l /\ mem e1 (project i (append tr op1)).l /\ 
+                        get_id e <> get_id e1 /\ (project i (append tr op1)).vis e e1 <==> 
+                 mem e (project i tr).l /\ mem e1 (project i tr).l /\ get_id e <> get_id e1 /\ (project i tr).vis e e1) /\
+                   (get_val_s #st1 #o i (app_op_a st op1) = (get_val_s #st1 #o i st))) ==>
+                     (sim #st1 #o) (project i (append tr op1)) (get_val_s #st1 #o i (app_op_a st op1))))
+
+#set-options "--z3rlimit 10000000"
+let lemma1 #st1 #o tr st op = admit ()
+
+val prop_oper3 : #st1:eqtype -> #o:eqtype -> {|mrdt st1 o|}
+               -> tr:ae (op o)
+               -> st:s st1
+               -> op1:(nat * (op o)) 
+               -> Lemma (requires (sim_a tr st) /\ (not (mem_id (get_id op1) tr.l)) /\
+                                 (forall e. mem e tr.l ==> get_id e < get_id op1) /\ get_id op1 > 0 /\
+                                 pre_cond_op #st1 #o (get_val_s #st1 #o (get_key op1) st) (project_op op1))
+                       (ensures (forall ch. mem_key_s ch (app_op_a st op1) /\ ch <> get_key op1 ==>
+                         (sim #st1 #o) (project ch (append tr op1)) (get_val_s #st1 #o ch (app_op_a st op1))))
+
+#set-options "--z3rlimit 10000000"
+let prop_oper3 #st1 #o tr st op = 
+  lem_oper tr op;
+  prop_oper1 tr st op;
+  prop_oper2 tr st op;
+  lemma1 #st1 #o tr st op
+
+val prop_oper_a : #st1:eqtype -> #o:eqtype -> {|mrdt st1 o|}
+                -> tr:ae (op o)
+                -> st:s st1
+                -> op1:(nat * (op o)) 
+                -> Lemma (requires (sim_a tr st) /\ (not (mem_id (get_id op1) tr.l)) /\
+                                  (forall e. mem e tr.l ==> get_id e < get_id op1) /\ get_id op1 > 0 /\
+                                  pre_cond_op #st1 #o (get_val_s #st1 #o (get_key op1) st) (project_op op1) /\
+     ((sim #st1 #o) (project (get_key op1) (append tr op1)) (get_val_s #st1 #o (get_key op1) (app_op_a st op1))))
+                      (ensures (sim_a (append tr op1) (app_op_a st op1)))
+
+#set-options "--z3rlimit 10000000"
+let prop_oper_a #st1 #o tr st op = 
+  lem_oper tr op;
+  prop_oper1 tr st op;
+  prop_oper2 tr st op;
+  prop_oper3 #st1 #o tr st op
+
+val get_key_lst : #st:eqtype 
+                -> l:s st -> a:s st -> b:s st
+                -> Pure (list nat)
+                  (requires true)
+                  (ensures (fun r -> (forall i. mem i r <==> mem_key_s i a \/ mem_key_s i b) /\ unique_keys r))
+                  (decreases %[l;a;b])
+
+let rec get_key_lst #st l a b =
+  match l,a,b with
+  |[],[],[] -> []
+  |x::xs,_,_ -> get_key_lst xs a b
+  |[],x::xs,_ -> if (mem_key_s (get_key_s x) b) then get_key_lst [] xs b else (get_key_s x)::(get_key_lst [] xs b)
+  |[],[],x::xs -> (get_key_s x)::(get_key_lst [] [] xs)
+
+val pre_cond_merge1_a : #st:eqtype -> #o:eqtype -> {|mrdt st o|}
+                      -> l:s st -> a:s st -> b:s st 
+                      -> Tot (b1:bool {b1=true <==> (forall e. mem_key_s e l ==> mem_key_s e a /\ mem_key_s e b) /\
+                        (forall ch. mem_key_s ch a \/ mem_key_s ch b ==> 
+                pre_cond_merge1 #st #o (get_val_s #st #o ch l) (get_val_s #st #o ch a) (get_val_s #st #o ch b))})
+let pre_cond_merge1_a #st #o l a b =
+  forallb (fun e -> mem_key_s (get_key_s #st e) a && mem_key_s (get_key_s #st e) b) l &&
+  forallb (fun ch -> pre_cond_merge1 #st #o (get_val_s #st #o ch l) 
+             (get_val_s #st #o ch a) (get_val_s #st #o ch b)) (get_key_lst l a b)
+
+val remove_key : #st:eqtype 
+               -> ch:nat
+               -> a:s st
+               -> Pure (s st)
+                 (requires (mem_key_s ch a))
+                 (ensures (fun r -> (forall i. mem_key_s i r <==> mem_key_s i a /\ ch <> i) /\
+                                 (forall e. mem e r <==> mem e a /\ get_key_s e <> ch)))
+let rec remove_key #st ch a =
+  match a with
+  |(ch1,v)::xs -> if ch = ch1 then xs else (ch1,v)::remove_key ch xs
+
+val merge2 : #st:eqtype -> #o:eqtype -> {|mrdt st o|}
+           -> l:s st
+           -> a:s st
+           -> b:s st
+           -> lst:list nat
+           -> Pure (s st)
+                (requires pre_cond_merge1_a #st #o l a b /\ unique_keys lst /\
+                          (forall ch. mem ch lst ==> mem_key_s ch a \/ mem_key_s ch b))
+                (ensures (fun r -> (forall ch. mem_key_s ch r <==> mem ch lst) /\ unique_key r /\
+                         (forall ch. mem ch lst ==> (get_val_s #st #o ch r) =
+                         (merge1 #st #o (get_val_s #st #o ch l) (get_val_s #st #o ch a) (get_val_s #st #o ch b)))))
+                (decreases lst)
+
+#set-options "--z3rlimit 10000000" 
+let rec merge2 #st #o l a b lst =
+  match lst with
+  |[] -> []
+  |x::xs -> (x, merge1 #st #o (get_val_s #st #o x l) (get_val_s #st #o x a) (get_val_s #st #o x b))::merge2 #st #o l a b xs
+
+val merge1_a : #st:eqtype -> #o:eqtype -> {|mrdt st o|}
+             -> l:s st
+             -> a:s st
+             -> b:s st
+             -> Pure (s st)
+               (requires pre_cond_merge1_a #st #o l a b)
+               (ensures (fun r -> (forall ch. mem_key_s ch r <==> mem_key_s ch a \/ mem_key_s ch b) /\ unique_key r /\
+                               (forall ch. mem_key_s ch a \/ mem_key_s ch b ==> (get_val_s #st #o ch r) =
+                      (merge1 #st #o (get_val_s #st #o ch l) (get_val_s #st #o ch a) (get_val_s #st #o ch b)))))
+
+#set-options "--z3rlimit 10000000" 
+let merge1_a #st #o l a b = 
+ let lst = get_key_lst l a b in
+ merge2 #st #o l a b lst
+
+val lem_merge1 : #st:eqtype -> #o:eqtype -> {|mrdt st o|}
+               -> ltr:ae (op o)
+               -> l:s st
+               -> atr:ae (op o)
+               -> a:s st
+               -> btr:ae (op o)
+               -> b:s st
+               -> lst:list nat
+               -> Lemma (requires (forall e. mem e ltr.l ==> not (mem_id (get_id e) atr.l)) /\
+                                 (forall e. mem e atr.l ==> not (mem_id (get_id e) btr.l)) /\
+                                 (forall e. mem e ltr.l ==> not (mem_id (get_id e) btr.l)) /\
+                                 (sim_a ltr l /\ sim_a (union ltr atr) a /\ sim_a (union ltr btr) b) /\
+                                 (forall ch. mem ch lst <==> mem_key_s ch a \/ mem_key_s ch b) /\ unique_keys lst)
+                       (ensures (forall i. mem_key_s i l ==> mem_key_s i a /\ mem_key_s i b))
+
+#set-options "--z3rlimit 10000000"
+let lem_merge1 ltr l atr a btr b lst = ()
+
+(*)val pre_cond_merge_a : #st:eqtype -> #o:eqtype -> {|mrdt st o|}
+            -> ltr:ae (op o) -> l:s st -> atr:ae (op o) -> a:s st -> btr:ae (op o) -> b:s st
+            -> Tot bool
+let pre_cond_merge_a ltr l atr a btr b = true*)
+
+val merge_a : #st:eqtype -> #o:eqtype -> {|mrdt st o|}
+            -> ltr:ae (op o)
+            -> l:s st
+            -> atr:ae (op o)
+            -> a:s st
+            -> btr:ae (op o)
+            -> b:s st
+            -> Pure (s st) 
+              (requires (forall e. mem e ltr.l ==> not (mem_id (get_id e) atr.l)) /\
+                        (forall e. mem e atr.l ==> not (mem_id (get_id e) btr.l)) /\
+                        (forall e. mem e ltr.l ==> not (mem_id (get_id e) btr.l)) /\
+                        (sim_a ltr l /\ sim_a (union ltr atr) a /\ sim_a (union ltr btr) b) /\ pre_cond_merge1_a #st #o l a b /\
+                        (forall ch. mem_key_s ch a \/ mem_key_s ch b ==> 
+                        (pre_cond_merge #st #o (project ch ltr) (get_val_s #st #o ch l)
+                                               (project ch atr) (get_val_s #st #o ch a)
+                                               (project ch btr) (get_val_s #st #o ch b)) /\
+                        (forall e. mem e (project ch ltr).l ==> not (mem_id (get_id e) (project ch atr).l)) /\
+                        (forall e. mem e (project ch atr).l ==> not (mem_id (get_id e) (project ch btr).l)) /\
+                        (forall e. mem e (project ch ltr).l ==> not (mem_id (get_id e) (project ch btr).l)) /\
+                        (sim #st #o (project ch ltr) (get_val_s #st #o ch l) /\ sim #st #o (union (project ch ltr) (project ch atr)) (get_val_s #st #o ch a) /\ sim #st #o (union (project ch ltr) (project ch btr)) (get_val_s #st #o ch b))))
+
+              (ensures (fun r -> (forall i. mem_key_s i l ==> mem_key_s i a /\ mem_key_s i b) /\
+                              (forall i. mem_key_s i r <==> mem_key_s i a \/ mem_key_s i b) /\
+                              (forall ch. mem_key_s ch r ==> (get_val_s #st #o ch r) =
+                    (merge1 #st #o (get_val_s #st #o ch l) (get_val_s #st #o ch a) (get_val_s #st #o ch b))) /\
+                         (forall ch. mem_key_s ch r ==> (get_val_s #st #o ch r) =
+                  (merge #st #o (project ch ltr) (get_val_s #st #o ch l) (project ch atr) (get_val_s #st #o ch a) (project ch btr) (get_val_s #st #o ch b))) /\ (r = merge1_a #st #o l a b)))
+
+let merge_a #st #o ltr l atr a btr b = 
+  let keys = get_key_lst l a b in
+  lem_merge1 ltr l atr a btr b keys;
+  let r = merge1_a #st #o l a b in
+  r
+
+val lemma6 : #o:eqtype 
+           -> l:ae (op o)
+           -> a:ae (op o)
+           -> Lemma (requires (forall e. mem e l.l ==> not (mem_id (get_id e) a.l)))
+                   (ensures (forall e. mem_op e (union1 l a) <==> mem_op e l.l \/ mem_op e a.l))
+                   (decreases %[l.l;a.l])
+
+#set-options "--z3rlimit 10000000"
+let rec lemma6 #o l a = 
+  match l,a with
+  |(A _ []), (A _ []) -> ()
+  |(A _ (x::xs)), _ -> lemma6 (A l.vis xs) a
+  |(A _ []), (A _ (x::xs)) -> lemma6 l (A a.vis xs)
+
+val lemma61 : #o:eqtype 
+            -> l:ae (op o)
+            -> a:ae (op o)
+            -> b:ae (op o)
+                 -> Lemma (requires (forall e. mem e l.l ==> not (mem_id (get_id e) a.l)) /\
+                                   (forall e. mem e a.l ==> not (mem_id (get_id e) b.l)) /\
+                                   (forall e. mem e l.l ==> not (mem_id (get_id e) b.l)))
+                         (ensures (forall e. mem_op e (absmerge1 l a b) <==> 
+                                        mem_op e l.l \/ mem_op e a.l \/ mem_op e b.l))
+                         (decreases %[l.l;a.l;b.l])
+
+#set-options "--z3rlimit 10000000"
+let rec lemma61 #o l a b = 
+  match l,a,b with
+  |(A _ []), (A _ []), (A _ []) -> ()
+  |(A _ (x::xs)), _, _ -> lemma61 (A l.vis xs) a b
+  |(A _ []), (A _ (x::xs)), _ -> lemma61 l (A a.vis xs) b
+  |(A _ []), (A _ []), (A _ (x::xs)) -> lemma61 l a (A b.vis xs)
+
+val lemma7 : #st:eqtype -> #o:eqtype -> {|mrdt st o|}
+           -> tr:ae o -> s1:st -> tr1:ae o
+           -> Lemma (requires sim tr s1 /\ (forall e. mem e tr1.l <==> mem e tr.l) /\
+                             (forall e e1. mem e tr1.l /\ mem e1 tr1.l /\ get_id e <> get_id e1 /\ tr1.vis e e1 <==>
+                                      mem e tr.l /\ mem e1 tr.l /\ get_id e <> get_id e1 /\ tr.vis e e1))
+                   (ensures (sim tr1 s1))
+let lemma7 #st #o tr s1 tr1 = admit ()
+
+val lemma8 : #o:eqtype 
+           -> ltr:ae (op o)
+           -> atr:ae (op o)
+           -> Lemma (requires (forall e. mem e ltr.l ==> not (mem_id (get_id e) atr.l)) /\
+                             (forall i e. mem e (project i ltr).l ==> not (mem_id (get_id e) (project i atr).l)))
+                   (ensures (forall i e. mem e (union (project i ltr) (project i atr)).l <==>
+                                    mem e (project i (union ltr atr)).l) /\
+                            (forall i. (forall e e1. (mem e (union (project i ltr) (project i atr)).l /\ 
+             mem e1 (union (project i ltr) (project i atr)).l /\ get_id e <> get_id e1 /\ 
+                    (union (project i ltr) (project i atr)).vis e e1) <==>
+            (mem e (project i (union ltr atr)).l /\ mem e1 (project i (union ltr atr)).l /\ get_id e <> get_id e1 /\
+                   (project i (union ltr atr)).vis e e1))))
+
+#set-options "--z3rlimit 10000000"
+let lemma8 #o ltr atr = ()
+
+val lemma9 : #o:eqtype
+           -> ltr:ae (op o)
+           -> atr:ae (op o)
+           -> btr:ae (op o)
+           -> Lemma (requires (forall e. mem e ltr.l ==> not (mem_id (get_id e) atr.l)) /\
+                             (forall e. mem e atr.l ==> not (mem_id (get_id e) btr.l)) /\
+                             (forall e. mem e ltr.l ==> not (mem_id (get_id e) btr.l))/\
+                             (forall i e. mem e (project i ltr).l ==> not (mem_id (get_id e) (project i atr).l)) /\
+                             (forall i e. mem e (project i atr).l ==> not (mem_id (get_id e) (project i btr).l)) /\
+                             (forall i e. mem e (project i ltr).l ==> not (mem_id (get_id e) (project i btr).l)))
+                   (ensures (forall i. (forall e. mem e (absmerge (project i ltr) (project i atr) (project i btr)).l <==>
+                             mem e (project i (absmerge ltr atr btr)).l)) /\
+             (forall i. (forall e e1. mem e (absmerge (project i ltr) (project i atr) (project i btr)).l /\
+                  mem e1 (absmerge (project i ltr) (project i atr) (project i btr)).l /\ get_id e <> get_id e1 /\
+                              (absmerge (project i ltr) (project i atr) (project i btr)).vis e e1 <==>
+                                mem e (project i (absmerge ltr atr btr)).l /\ mem e1 (project i (absmerge ltr atr btr)).l /\ get_id e <> get_id e1 /\ (project i (absmerge ltr atr btr)).vis e e1)))
+
+#set-options "--z3rlimit 10000000"
+let lemma9 #o ltr atr btr = ()
+
+val prop_merge1 : #st:eqtype -> #o:eqtype -> {|mrdt st o|}
+                -> ltr:ae (op o)
+                -> l:s st
+                -> atr:ae (op o)
+                -> a:s st
+                -> btr:ae (op o)
+                -> b:s st
+                -> chs:list nat
+                -> Lemma (requires (forall e. mem e ltr.l ==> not (mem_id (get_id e) atr.l)) /\
+                                  (forall e. mem e atr.l ==> not (mem_id (get_id e) btr.l)) /\
+                                  (forall e. mem e ltr.l ==> not (mem_id (get_id e) btr.l)) /\
+                                  (forall i e. mem e (project i ltr).l ==> not (mem_id (get_id e) (project i atr).l)) /\
+                                  (forall i e. mem e (project i atr).l ==> not (mem_id (get_id e) (project i btr).l)) /\
+                                  (forall i e. mem e (project i ltr).l ==> not (mem_id (get_id e) (project i btr).l)) /\
+                                  (sim_a ltr l /\ sim_a (union ltr atr) a /\ sim_a (union ltr btr) b) /\
+                                  (forall i. mem_key_s i l ==> mem_key_s i a /\ mem_key_s i b) /\
+                                  (forall i. mem i chs ==> mem_key_s i a \/ mem_key_s i b) /\
+                                  pre_cond_merge1_a #st #o l a b /\
+                                  (forall i. mem_key_s i a \/ mem_key_s i b ==> 
+                                  pre_cond_merge #st #o (project i ltr) (get_val_s #st #o i l)
+                                                           (project i atr) (get_val_s #st #o i a)
+                                                           (project i btr) (get_val_s #st #o i b) /\
+                                  (forall e. mem e (project i ltr).l ==> not (mem_id (get_id e) (project i atr).l)) /\
+                                  (forall e. mem e (project i atr).l ==> not (mem_id (get_id e) (project i btr).l)) /\
+                                  (forall e. mem e (project i ltr).l ==> not (mem_id (get_id e) (project i btr).l)) /\
+                                  (sim #st #o (project i ltr) (get_val_s #st #o i l) /\ sim #st #o (union (project i ltr) (project i atr)) (get_val_s #st #o i a) /\ sim #st #o (union (project i ltr) (project i btr)) (get_val_s #st #o i b))) /\
+                                  (forall i. mem i chs ==> mem_key_s i (merge_a ltr l atr a btr b)))
+                        (ensures (forall i. mem i chs ==> 
+             ((sim #st #o) (project i (absmerge ltr atr btr)) (get_val_s #st #o i (merge_a ltr l atr a btr b)))))
+                        (decreases chs)
+
+#set-options "--z3rlimit 10000000"
+let rec prop_merge1 #st #o ltr l atr a btr b lst =
+  match lst with
+  |[] -> ()
+  |i::is -> lemma4 #st #o ltr l; lemma4 #st #o (union ltr atr) a; lemma4 #st #o (union ltr btr) b;
+          lemma8 #o ltr atr; lemma8 #o ltr btr; 
+          lemma7 #st #o (project i (union ltr atr)) (get_val_s #st #o i a) (union (project i ltr) (project i atr));
+          lemma7 #st #o (project i (union ltr btr)) (get_val_s #st #o i b) (union (project i ltr) (project i btr));
+          (prop_merge #st #o) (project i ltr) (get_val_s #st #o i l) (project i atr) (get_val_s #st #o i a) (project i btr) (get_val_s #st #o i b);
+          assert (sim #st #o (absmerge (project i ltr) (project i atr) (project i btr)) (merge #st #o (project i ltr) (get_val_s #st #o i l) (project i atr) (get_val_s #st #o i a) (project i btr) (get_val_s #st #o i b)));
+          lemma9 #o ltr atr btr;
+          assert ((sim #st #o) (absmerge (project i ltr) (project i atr) (project i btr)) (get_val_s #st #o i (merge_a ltr l atr a btr b))); 
+          lemma7 #st #o (absmerge (project i ltr) (project i atr) (project i btr)) 
+                 (get_val_s #st #o i (merge_a ltr l atr a btr b)) (project i (absmerge ltr atr btr)); 
+          assert ((sim #st #o) (project i (absmerge ltr atr btr)) (get_val_s #st #o i (merge_a ltr l atr a btr b)));
+          prop_merge1 #st #o ltr l atr a btr b is
+
+val prop_merge21 : #st:eqtype -> #o:eqtype -> {|mrdt st o|}
+          -> ltr:ae (op o)
+          -> l:s st
+          -> atr:ae (op o)
+          -> a:s st
+          -> btr:ae (op o)
+          -> b:s st
+          -> Lemma (requires (forall e. mem e ltr.l ==> not (mem_id (get_id e) atr.l)) /\
+                            (forall e. mem e atr.l ==> not (mem_id (get_id e) btr.l)) /\
+                            (forall e. mem e ltr.l ==> not (mem_id (get_id e) btr.l)) /\
+                            (sim_a ltr l /\ sim_a (union ltr atr) a /\ sim_a (union ltr btr) b) /\
+                             pre_cond_merge1_a #st #o l a b /\
+                            (forall ch. mem_key_s ch a \/ mem_key_s ch b ==> 
+                            (pre_cond_merge #st #o (project ch ltr) (get_val_s #st #o ch l)
+                                                   (project ch atr) (get_val_s #st #o ch a)
+                                                   (project ch btr) (get_val_s #st #o ch b)) /\
+                            (forall e. mem e (project ch ltr).l ==> not (mem_id (get_id e) (project ch atr).l)) /\
+                            (forall e. mem e (project ch atr).l ==> not (mem_id (get_id e) (project ch btr).l)) /\
+                            (forall e. mem e (project ch ltr).l ==> not (mem_id (get_id e) (project ch btr).l)) /\
+                            (sim #st #o (project ch ltr) (get_val_s #st #o ch l) /\ sim #st #o (union (project ch ltr) (project ch atr)) (get_val_s #st #o ch a) /\ sim #st #o (union (project ch ltr) (project ch btr)) (get_val_s #st #o ch b))))
+                  (ensures (forall e. mem e (merge_a ltr l atr a btr b) ==> mem_key (get_key_s e) (absmerge ltr atr btr).l))
+
+#set-options "--z3rlimit 10000000"
+let prop_merge21 #st #o ltr l atr a btr b = 
+  lemma2 #st #o (merge_a ltr l atr a btr b);
+  lemma6 ltr atr; lemma6 ltr btr;
+  lemma61 ltr atr btr
+
+val prop_merge22 : #st:eqtype -> #o:eqtype -> {|mrdt st o|}
+          -> ltr:ae (op o)
+          -> l:s st
+          -> atr:ae (op o)
+          -> a:s st
+          -> btr:ae (op o)
+          -> b:s st
+          -> Lemma (requires (forall e. mem e ltr.l ==> not (mem_id (get_id e) atr.l)) /\
+                            (forall e. mem e atr.l ==> not (mem_id (get_id e) btr.l)) /\
+                            (forall e. mem e ltr.l ==> not (mem_id (get_id e) btr.l)) /\
+                            (sim_a ltr l /\ sim_a (union ltr atr) a /\ sim_a (union ltr btr) b) /\
+                             pre_cond_merge1_a #st #o l a b /\
+                            (forall ch. mem_key_s ch a \/ mem_key_s ch b ==> 
+                            (pre_cond_merge #st #o (project ch ltr) (get_val_s #st #o ch l)
+                                                   (project ch atr) (get_val_s #st #o ch a)
+                                                   (project ch btr) (get_val_s #st #o ch b)) /\
+                            (forall e. mem e (project ch ltr).l ==> not (mem_id (get_id e) (project ch atr).l)) /\
+                            (forall e. mem e (project ch atr).l ==> not (mem_id (get_id e) (project ch btr).l)) /\
+                            (forall e. mem e (project ch ltr).l ==> not (mem_id (get_id e) (project ch btr).l)) /\
+                            (sim #st #o (project ch ltr) (get_val_s #st #o ch l) /\ sim #st #o (union (project ch ltr) (project ch atr)) (get_val_s #st #o ch a) /\ sim #st #o (union (project ch ltr) (project ch btr)) (get_val_s #st #o ch b))))
+                   (ensures (forall e. mem e (absmerge ltr atr btr).l ==> 
+                                      mem_key_s (get_key e) (merge_a ltr l atr a btr b)))
+
+#set-options "--z3rlimit 10000000"
+let prop_merge22 #st #o ltr l atr a btr b = 
+  lemma2 #st #o (merge_a ltr l atr a btr b);
+  lemma6 ltr atr; lemma6 ltr btr;
+  lemma61 ltr atr btr
+
+val prop_merge2 : #st:eqtype -> #o:eqtype -> {|mrdt st o|}
+          -> ltr:ae (op o)
+          -> l:s st
+          -> atr:ae (op o)
+          -> a:s st
+          -> btr:ae (op o)
+          -> b:s st
+          -> Lemma (requires (forall e. mem e ltr.l ==> not (mem_id (get_id e) atr.l)) /\
+                            (forall e. mem e atr.l ==> not (mem_id (get_id e) btr.l)) /\
+                            (forall e. mem e ltr.l ==> not (mem_id (get_id e) btr.l)) /\
+                            (sim_a ltr l /\ sim_a (union ltr atr) a /\ sim_a (union ltr btr) b) /\
+                             pre_cond_merge1_a #st #o l a b /\
+                            (forall ch. mem_key_s ch a \/ mem_key_s ch b ==> 
+                            (pre_cond_merge #st #o (project ch ltr) (get_val_s #st #o ch l)
+                                                   (project ch atr) (get_val_s #st #o ch a)
+                                                   (project ch btr) (get_val_s #st #o ch b)) /\
+                            (forall e. mem e (project ch ltr).l ==> not (mem_id (get_id e) (project ch atr).l)) /\
+                            (forall e. mem e (project ch atr).l ==> not (mem_id (get_id e) (project ch btr).l)) /\
+                            (forall e. mem e (project ch ltr).l ==> not (mem_id (get_id e) (project ch btr).l)) /\
+                            (sim #st #o (project ch ltr) (get_val_s #st #o ch l) /\ sim #st #o (union (project ch ltr) (project ch atr)) (get_val_s #st #o ch a) /\ sim #st #o (union (project ch ltr) (project ch btr)) (get_val_s #st #o ch b))))
+                   (ensures (forall ch. mem_key_s ch (merge_a ltr l atr a btr b) <==> 
+                                       mem_key ch (absmerge ltr atr btr).l))
+
+#set-options "--z3rlimit 10000000"
+let prop_merge2 #st #o ltr l atr a btr b = 
+  prop_merge21 #st #o ltr l atr a btr b;
+  prop_merge22 #st #o ltr l atr a btr b
+
+val prop_merge31 : #st:eqtype -> #o:eqtype -> {|mrdt st o|}
+          -> ltr:ae (op o)
+          -> l:s st
+          -> atr:ae (op o)
+          -> a:s st
+          -> btr:ae (op o)
+          -> b:s st
+          -> Lemma (requires (forall e. mem e ltr.l ==> not (mem_id (get_id e) atr.l)) /\
+                            (forall e. mem e atr.l ==> not (mem_id (get_id e) btr.l)) /\
+                            (forall e. mem e ltr.l ==> not (mem_id (get_id e) btr.l)) /\
+                            (sim_a ltr l /\ sim_a (union ltr atr) a /\ sim_a (union ltr btr) b) /\
+                             pre_cond_merge1_a #st #o l a b /\
+                            (forall ch. mem_key_s ch a \/ mem_key_s ch b ==> 
+                            (pre_cond_merge #st #o (project ch ltr) (get_val_s #st #o ch l)
+                                                   (project ch atr) (get_val_s #st #o ch a)
+                                                   (project ch btr) (get_val_s #st #o ch b)) /\
+                            (forall e. mem e (project ch ltr).l ==> not (mem_id (get_id e) (project ch atr).l)) /\
+                            (forall e. mem e (project ch atr).l ==> not (mem_id (get_id e) (project ch btr).l)) /\
+                            (forall e. mem e (project ch ltr).l ==> not (mem_id (get_id e) (project ch btr).l)) /\
+                            (sim #st #o (project ch ltr) (get_val_s #st #o ch l) /\ sim #st #o (union (project ch ltr) (project ch atr)) (get_val_s #st #o ch a) /\ sim #st #o (union (project ch ltr) (project ch btr)) (get_val_s #st #o ch b))) /\ (forall ch. mem_key_s ch (merge_a ltr l atr a btr b) <==> mem_key ch (absmerge ltr atr btr).l))
+                    (ensures (forall e. mem e (absmerge ltr atr btr).l ==> 
+                             (exists e1. mem e1 (merge_a ltr l atr a btr b) /\ get_key e = get_key_s e1)))
+
+#set-options "--z3rlimit 10000000"
+let prop_merge31 #st #o ltr l atr a btr b = 
+  lemma2 #st #o (merge_a ltr l atr a btr b);
+  lemma6 ltr atr; lemma6 ltr btr;
+  lemma61 ltr atr btr
+  
+val prop_merge_a : #st:eqtype -> #o:eqtype -> {|mrdt st o|}
+          -> ltr:ae (op o)
+          -> l:s st
+          -> atr:ae (op o)
+          -> a:s st
+          -> btr:ae (op o)
+          -> b:s st
+          -> Lemma (requires (forall e. mem e ltr.l ==> not (mem_id (get_id e) atr.l)) /\
+                            (forall e. mem e atr.l ==> not (mem_id (get_id e) btr.l)) /\
+                            (forall e. mem e ltr.l ==> not (mem_id (get_id e) btr.l)) /\
+                            (sim_a ltr l /\ sim_a (union ltr atr) a /\ sim_a (union ltr btr) b) /\
+                             pre_cond_merge1_a #st #o l a b /\
+                            (forall ch. mem_key_s ch a \/ mem_key_s ch b ==> 
+                            (pre_cond_merge #st #o (project ch ltr) (get_val_s #st #o ch l)
+                                                   (project ch atr) (get_val_s #st #o ch a)
+                                                   (project ch btr) (get_val_s #st #o ch b)) /\
+                            (forall e. mem e (project ch ltr).l ==> not (mem_id (get_id e) (project ch atr).l)) /\
+                            (forall e. mem e (project ch atr).l ==> not (mem_id (get_id e) (project ch btr).l)) /\
+                            (forall e. mem e (project ch ltr).l ==> not (mem_id (get_id e) (project ch btr).l)) /\
+                            (sim #st #o (project ch ltr) (get_val_s #st #o ch l) /\ sim #st #o (union (project ch ltr) (project ch atr)) (get_val_s #st #o ch a) /\ sim #st #o (union (project ch ltr) (project ch btr)) (get_val_s #st #o ch b))))
+                    (ensures (sim_a (absmerge ltr atr btr) (merge_a ltr l atr a btr b)))
+
+#set-options "--z3rlimit 10000000"
+let prop_merge_a #st #o ltr l atr a btr b = 
+  prop_merge2 #st #o ltr l atr a btr b;
+  prop_merge31 #st #o ltr l atr a btr b;
+  let m = get_lst (merge_a ltr l atr a btr b) in
+  prop_merge1 #st #o ltr l atr a btr b m
+
+
