log_map.fst
@@ -1,0 +1,290 @@
+module Log_map
+open FStar.List.Tot
+
+open Library
+open FStar.Tactics.Typeclasses
+
+module A = Alpha_map
+
+module G = Log
+
+val pre_cond_merge1_a1 : l:A.s G.s -> a:A.s G.s -> b:A.s G.s 
+                      -> Pure bool
+                        (requires true)
+                        (ensures (fun b1 -> (b1 = true <==> (forall e. A.mem_key_s e l ==> A.mem_key_s e a /\ A.mem_key_s e b) /\
+                        (forall ch. A.mem_key_s ch a \/ A.mem_key_s ch b ==> 
+                                       (forall e. mem e (A.get_val_s #G.s #G.op ch l) ==> mem e (A.get_val_s #G.s #G.op ch a) /\ mem e (A.get_val_s #G.s #G.op ch b)) /\
+                      (forall e e1. mem e (A.get_val_s #G.s #G.op ch l) /\ mem e1 (G.diff_s (A.get_val_s #G.s #G.op ch a) (A.get_val_s #G.s #G.op ch l)) ==> G.fst e1 > G.fst e) /\
+                      (forall e e1. mem e (A.get_val_s #G.s #G.op ch l) /\ mem e1 (G.diff_s (A.get_val_s #G.s #G.op ch b) (A.get_val_s #G.s #G.op ch l)) ==> G.fst e1 > G.fst e)))))
+
+#set-options "--z3rlimit 10000000"
+let pre_cond_merge1_a1 l a b =
+  forallb (fun e -> A.mem_key_s (A.get_key_s #G.s e) a && A.mem_key_s (A.get_key_s #G.s e) b) l &&
+  forallb (fun ch -> (forallb (fun e -> mem e (A.get_val_s #G.s #G.op ch a) && mem e (A.get_val_s #G.s #G.op ch b)) (A.get_val_s #G.s #G.op ch l)) &&
+            (forallb (fun e -> (forallb (fun e1 -> G.fst e1 > G.fst e) (G.diff_s (A.get_val_s #G.s #G.op ch a) (A.get_val_s #G.s #G.op ch l)))) (A.get_val_s #G.s #G.op ch l)) &&
+            (forallb (fun e -> (forallb (fun e1 -> G.fst e1 > G.fst e) (G.diff_s (A.get_val_s #G.s #G.op ch b) (A.get_val_s #G.s #G.op ch l)))) (A.get_val_s #G.s #G.op ch l))) (A.get_key_lst l a b)
+
+val pre_cond_merge1_a2 : l:A.s G.s -> a:A.s G.s -> b:A.s G.s 
+                      -> Pure bool
+                        (requires true)
+                        (ensures (fun b1 -> (b1 = true <==> (forall ch. A.mem_key_s ch a \/ A.mem_key_s ch b ==> 
+                                           (G.pre_cond_merge1 (A.get_val_s #G.s #G.op ch l) 
+                                           (A.get_val_s #G.s #G.op ch a) (A.get_val_s #G.s #G.op ch b)) /\
+                        (forall e. mem e (A.get_val_s #G.s #G.op ch l) ==> mem e (A.get_val_s #G.s #G.op ch a) /\ mem e (A.get_val_s #G.s #G.op ch b)) /\
+                          (forall e. mem e (G.diff_s (A.get_val_s #G.s #G.op ch a) (A.get_val_s #G.s #G.op ch l)) ==>
+                      not (G.mem_id_s (G.fst e) (G.diff_s (A.get_val_s #G.s #G.op ch b) (A.get_val_s #G.s #G.op ch l)))) /\
+                      (forall e. mem e (G.diff_s (A.get_val_s #G.s #G.op ch b) (A.get_val_s #G.s #G.op ch l)) ==>
+                                                         not (G.mem_id_s (G.fst e) (G.diff_s (A.get_val_s #G.s #G.op ch a) (A.get_val_s#G.s #G.op  ch l))))))))
+
+#set-options "--z3rlimit 10000000"
+let pre_cond_merge1_a2 l a b =
+  forallb (fun ch -> G.pre_cond_merge1 (A.get_val_s #G.s #G.op ch l) (A.get_val_s #G.s #G.op ch a) (A.get_val_s #G.s #G.op ch b) &&
+            (forallb (fun e -> mem e (A.get_val_s #G.s #G.op ch a) && mem e (A.get_val_s #G.s #G.op ch b)) (A.get_val_s #G.s #G.op ch l)) &&
+
+            (forallb (fun e -> not (G.mem_id_s (G.fst e) (G.diff_s (A.get_val_s #G.s #G.op ch b) (A.get_val_s #G.s #G.op ch l)))) (G.diff_s (A.get_val_s #G.s #G.op ch a) (A.get_val_s #G.s #G.op ch l))) &&
+            (forallb (fun e -> not (G.mem_id_s (G.fst e) (G.diff_s (A.get_val_s #G.s #G.op ch a) (A.get_val_s#G.s #G.op  ch l)))) (G.diff_s (A.get_val_s #G.s #G.op ch b) (A.get_val_s #G.s #G.op ch l)))) (A.get_key_lst l a b)
+
+val pre_cond_merge1_a : l:A.s G.s -> a:A.s G.s -> b:A.s G.s 
+                      -> Pure bool
+                        (requires true)
+                        (ensures (fun b1 -> (b1 = true <==> (forall e. A.mem_key_s e l ==> A.mem_key_s e a /\ A.mem_key_s e b) /\
+                        (forall ch. A.mem_key_s ch a \/ A.mem_key_s ch b ==> 
+                                           (G.pre_cond_merge1 (A.get_val_s #G.s #G.op ch l) 
+                                           (A.get_val_s #G.s #G.op ch a) (A.get_val_s #G.s #G.op ch b)) /\
+                        (forall e. mem e (A.get_val_s #G.s #G.op ch l) ==> mem e (A.get_val_s #G.s #G.op ch a) /\ mem e (A.get_val_s #G.s #G.op ch b)) /\
+                          (forall e. mem e (G.diff_s (A.get_val_s #G.s #G.op ch a) (A.get_val_s #G.s #G.op ch l)) ==>
+                      not (G.mem_id_s (G.fst e) (G.diff_s (A.get_val_s #G.s #G.op ch b) (A.get_val_s #G.s #G.op ch l)))) /\
+                      (forall e. mem e (G.diff_s (A.get_val_s #G.s #G.op ch b) (A.get_val_s #G.s #G.op ch l)) ==>
+                                                         not (G.mem_id_s (G.fst e) (G.diff_s (A.get_val_s #G.s #G.op ch a) (A.get_val_s#G.s #G.op  ch l)))) /\
+                      (forall e e1. mem e (A.get_val_s #G.s #G.op ch l) /\ mem e1 (G.diff_s (A.get_val_s #G.s #G.op ch a) (A.get_val_s #G.s #G.op ch l)) ==> G.fst e1 > G.fst e) /\
+                      (forall e e1. mem e (A.get_val_s #G.s #G.op ch l) /\ mem e1 (G.diff_s (A.get_val_s #G.s #G.op ch b) (A.get_val_s #G.s #G.op ch l)) ==> G.fst e1 > G.fst e)))))
+
+#set-options "--z3rlimit 10000000"
+let pre_cond_merge1_a l a b =
+  pre_cond_merge1_a1 l a b &&
+  pre_cond_merge1_a2 l a b
+
+val merge2 : l:A.s G.s -> a:A.s G.s -> b:A.s G.s 
+           -> lst:list nat
+           -> Pure (A.s G.s)
+             (requires pre_cond_merge1_a l a b /\ A.unique_keys lst /\
+                       (forall ch. mem ch lst ==> A.mem_key_s ch a \/ A.mem_key_s ch b))
+             (ensures (fun r -> (forall ch. A.mem_key_s ch r <==> mem ch lst) /\ A.unique_key r /\
+                             (forall ch. mem ch lst ==> (A.get_val_s #G.s #G.op ch r) =
+                             (G.merge1 (A.get_val_s #G.s #G.op ch l) (A.get_val_s #G.s #G.op ch a) (A.get_val_s #G.s #G.op ch b)))))
+                (decreases lst)
+
+#set-options "--z3rlimit 10000000"
+let rec merge2 l a b lst =
+  match lst with
+  |[] -> []
+  |x::xs -> (x, G.merge1 (A.get_val_s #G.s #G.op x l) (A.get_val_s #G.s #G.op x a) (A.get_val_s #G.s #G.op x b))::merge2 l a b xs
+
+val merge1_a : l:A.s G.s
+             -> a:A.s G.s
+             -> b:A.s G.s
+             -> Pure (A.s G.s)
+               (requires pre_cond_merge1_a l a b)
+               (ensures (fun r -> (forall ch. A.mem_key_s ch r <==> A.mem_key_s ch a \/ A.mem_key_s ch b) /\ A.unique_key r /\
+                               (forall ch. A.mem_key_s ch a \/ A.mem_key_s ch b ==> (A.get_val_s #G.s #G.op ch r) =
+                               (G.merge1 (A.get_val_s #G.s #G.op ch l) (A.get_val_s #G.s #G.op ch a) (A.get_val_s #G.s #G.op ch b)))))
+
+let merge1_a l a b = 
+  let lst = A.get_key_lst l a b in
+  merge2 l a b lst
+
+val lemma2 : s1:A.s G.s
+           -> Lemma (requires true)
+                   (ensures (forall e. mem e s1 ==> (A.get_val_s #G.s #G.op (A.get_key_s e) s1 = A.get_val_s1 #G.s e)))
+let rec lemma2 s1 =
+  match s1 with
+  |[] -> ()
+  |x::xs -> lemma2 xs
+
+val lemma4 : tr:ae (A.op G.op) -> s1:A.s G.s
+           -> Lemma (requires A.sim_a tr s1)
+                   (ensures (forall i. (G.sim (A.project i tr) (A.get_val_s #G.s #G.op i s1))))
+let lemma4 tr s1 = ()
+
+val lemma1 : tr:ae (A.op G.op)
+         -> st:A.s G.s
+         -> op1:(nat * (A.op G.op))
+         -> Lemma (requires (A.sim_a tr st) /\ (not (mem_id (get_id op1) tr.l)) /\
+                           (forall e. mem e tr.l ==> get_id e < get_id op1) /\ get_id op1 > 0 /\
+                           G.pre_cond_op (A.get_val_s #G.s #G.op (A.get_key op1) st) (A.project_op op1))
+                 (ensures (forall i. A.mem_key_s i (A.app_op_a st op1) /\ i <> A.get_key op1 ==>
+                 ((forall e. mem e (A.project i (append tr op1)).l <==> mem e (A.project i tr).l) /\
+             (forall e e1. mem e (A.project i (append tr op1)).l /\ mem e1 (A.project i (append tr op1)).l /\ get_id e <> get_id e1 /\
+                      (A.project i (append tr op1)).vis e e1 <==> 
+                 mem e (A.project i tr).l /\ mem e1 (A.project i tr).l /\ get_id e <> get_id e1 /\ (A.project i tr).vis e e1) /\
+                   (A.get_val_s #G.s #G.op i (A.app_op_a st op1) = (A.get_val_s #G.s #G.op i st))) ==>
+                     (G.sim (A.project i (append tr op1)) (A.get_val_s #G.s #G.op i (A.app_op_a st op1)))))
+
+#set-options "--z3rlimit 10000000"
+let lemma1 tr st op = ()
+
+val lemma7 : tr:ae G.op -> s1:G.s -> tr1:ae G.op
+           -> Lemma (requires G.sim tr s1 /\ (forall e. mem e tr1.l <==> mem e tr.l) /\
+                             (forall e e1. mem e tr1.l /\ mem e1 tr1.l /\ get_id e <> get_id e1 /\ tr1.vis e e1 <==>
+                                      mem e tr.l /\ mem e1 tr.l /\ get_id e <> get_id e1 /\ tr.vis e e1))
+                   (ensures (G.sim tr1 s1))
+#set-options "--z3rlimit 10000000"
+let lemma7 tr s1 tr1 = ()
+
+val pre_cond_merge_a : ltr:ae (A.op G.op) 
+                     -> l:A.s G.s 
+                     -> atr:ae (A.op G.op)
+                     -> a:A.s G.s 
+                     -> btr:ae (A.op G.op)
+                     -> b:A.s G.s
+                     -> Tot (b1:bool {b1=true <==> (forall ch. A.mem_key_s ch a \/ A.mem_key_s ch b ==>
+                          (G.pre_cond_merge (A.project ch ltr) (A.get_val_s #G.s #G.op ch l)
+                                            (A.project ch atr) (A.get_val_s #G.s #G.op ch a)
+                                            (A.project ch btr) (A.get_val_s #G.s #G.op ch b)) /\
+                              (forall e. mem e (A.project ch ltr).l ==> not (mem_id (get_id e) (A.project ch atr).l)) /\
+                              (forall e. mem e (A.project ch atr).l ==> not (mem_id (get_id e) (A.project ch btr).l)) /\
+                              (forall e. mem e (A.project ch ltr).l ==> not (mem_id (get_id e) (A.project ch btr).l)) /\
+                              (G.sim (A.project ch ltr) (A.get_val_s #G.s #G.op ch l) /\ 
+                           G.sim (union (A.project ch ltr) (A.project ch atr)) (A.get_val_s #G.s #G.op ch a) /\
+                  G.sim (union (A.project ch ltr) (A.project ch btr)) (A.get_val_s #G.s #G.op ch b)))})
+
+let pre_cond_merge_a ltr l atr a btr b = 
+    forallb (fun ch -> (G.pre_cond_merge (A.project ch ltr) (A.get_val_s #G.s #G.op ch l)
+                                      (A.project ch atr) (A.get_val_s #G.s #G.op ch a)
+                                      (A.project ch btr) (A.get_val_s #G.s #G.op ch b)) &&
+                    (forallb (fun e -> not (mem_id (get_id e) (A.project ch atr).l)) (A.project ch ltr).l) &&
+                    (forallb (fun e -> not (mem_id (get_id e) (A.project ch btr).l)) (A.project ch atr).l) &&
+                    (forallb (fun e -> not (mem_id (get_id e) (A.project ch btr).l)) (A.project ch ltr).l) &&
+                    (G.sim (A.project ch ltr) (A.get_val_s #G.s #G.op ch l)) &&
+                    (G.sim (union (A.project ch ltr) (A.project ch atr)) (A.get_val_s #G.s #G.op ch a)) &&
+                    (G.sim (union (A.project ch ltr) (A.project ch btr)) (A.get_val_s #G.s #G.op ch b)))
+             (A.get_key_lst l a b)
+
+val merge_a : ltr:ae (A.op G.op)
+          -> l:A.s G.s
+          -> atr:ae (A.op G.op)
+          -> a:A.s G.s
+          -> btr:ae (A.op G.op)
+          -> b:A.s G.s
+          -> Pure (A.s G.s) (requires (forall e. mem e ltr.l ==> not (mem_id (get_id e) atr.l)) /\
+                             (forall e. mem e atr.l ==> not (mem_id (get_id e) btr.l)) /\
+                             (forall e. mem e ltr.l ==> not (mem_id (get_id e) btr.l)) /\
+                             (A.sim_a ltr l /\ A.sim_a (union ltr atr) a /\ A.sim_a (union ltr btr) b) /\
+                             pre_cond_merge1_a l a b /\ pre_cond_merge_a ltr l atr a btr b)
+                 (ensures (fun r -> (forall i. A.mem_key_s i l ==> A.mem_key_s i a /\ A.mem_key_s i b) /\
+                                 (forall i. A.mem_key_s i r <==> A.mem_key_s i a \/ A.mem_key_s i b) /\
+                               (forall ch. A.mem_key_s ch r ==> (A.get_val_s #G.s #G.op ch r) =
+      (G.merge1 (A.get_val_s #G.s #G.op ch l) (A.get_val_s #G.s #G.op ch a) (A.get_val_s #G.s #G.op ch b))) /\
+                             (forall ch. A.mem_key_s ch r ==> (A.get_val_s #G.s #G.op ch r) =
+                        (G.merge (A.project ch ltr) (A.get_val_s #G.s #G.op ch l) (A.project ch atr) (A.get_val_s #G.s #G.op ch a) (A.project ch btr) (A.get_val_s #G.s #G.op ch b))) /\
+                        (r = merge1_a l a b)))
+
+#set-options "--z3rlimit 10000000"
+let merge_a ltr l atr a btr b = 
+  let keys = A.get_key_lst l a b in
+  A.lem_merge1 ltr l atr a btr b keys;
+  let r = merge1_a l a b in
+  r
+
+val prop_oper : tr:ae (A.op G.op)
+              -> st:A.s G.s
+              -> op1:(nat * (A.op G.op)) 
+              -> Lemma (requires (A.sim_a tr st) /\ (not (mem_id (get_id op1) tr.l)) /\
+                                (forall e. mem e tr.l ==> get_id e < get_id op1) /\ get_id op1 > 0 /\
+                                A.pre_cond_op_a st op1)
+                      (ensures (A.sim_a (append tr op1) (A.app_op_a st op1)))
+
+#set-options "--z3rlimit 10000000"
+let prop_oper tr st op = 
+  assert (G.pre_cond_op (A.get_val_s #G.s #G.op (A.get_key op) st) (A.project_op op));
+  G.prop_oper (A.project (A.get_key op) tr) (A.get_val_s #G.s #G.op (A.get_key op) st) (A.project_op op); 
+  assert (G.sim (append (A.project (A.get_key op) tr) (A.project_op op)) (G.app_op (A.get_val_s #G.s #G.op (A.get_key op) st) (A.project_op op)));
+  A.lem_oper tr op;
+  assert (G.app_op (A.get_val_s #G.s #G.op (A.get_key op) st) (A.project_op op) =
+          A.get_val_s #G.s #G.op (A.get_key op) (A.app_op_a st op));
+  assert (G.sim (A.project (A.get_key op) (append tr op)) (A.get_val_s #G.s #G.op (A.get_key op) (A.app_op_a st op)));
+  A.prop_oper_a tr st op; ()
+
+val convergence2 : tr:ae (A.op G.op)
+                 -> a:(A.s G.s)
+                 -> b:(A.s G.s)
+                 -> Lemma (requires (A.sim_a tr a /\ A.sim_a tr b))
+                         (ensures (forall ch. A.mem_key_s ch a /\ A.mem_key_s ch b ==> 
+                             (forall e e1. mem e (A.get_val_s #G.s #G.op ch a) /\ mem e1 (A.get_val_s #G.s #G.op ch a) /\ 
+                              G.fst e <> G.fst e1 /\ G.fst e > G.fst e1 /\ G.ord e e1 (A.get_val_s #G.s #G.op ch a)  <==> 
+                  mem e (A.get_val_s #G.s #G.op ch b) /\ mem e1 (A.get_val_s #G.s #G.op ch b) /\ G.fst e <> G.fst e1 /\
+                                       G.fst e > G.fst e1 /\ G.ord e e1 (A.get_val_s #G.s #G.op ch b))) /\
+                                     (forall ch. A.mem_key_s ch a /\ A.mem_key_s ch b ==>
+                 (forall e. G.mem_id_s e (A.get_val_s #G.s #G.op ch a) <==> G.mem_id_s e (A.get_val_s #G.s #G.op ch b))))
+
+#set-options "--z3rlimit 100000000"
+let convergence2 tr a b = 
+  A.convergence_a1 tr a b
+
+val lem_length : a:(A.s G.s)
+               -> b:(A.s G.s)
+               -> lst:list nat
+               -> Lemma (requires (forall ch. mem ch lst ==> A.mem_key_s ch a /\ A.mem_key_s ch b) /\
+                                          (forall e. A.mem_key_s e a <==> A.mem_key_s e b) /\
+                                    A.unique_keys lst /\ (forall ch. mem ch lst ==> 
+                 (forall e. G.mem_id_s e (A.get_val_s #G.s #G.op ch a) <==> G.mem_id_s e (A.get_val_s #G.s #G.op ch b))))
+                 (ensures (forall ch. mem ch lst ==> (List.Tot.length (A.get_val_s #G.s #G.op ch a) = List.Tot.length (A.get_val_s #G.s #G.op ch b))))
+                          (decreases lst)
+
+let rec lem_length a b lst =
+  match lst with
+  |[] -> ()
+  |ch::chs -> G.lem_length (A.get_val_s #G.s #G.op ch a) (A.get_val_s #G.s #G.op ch b); lem_length a b chs
+
+val convergence3 : a:(A.s G.s)
+                 -> b:(A.s G.s)
+                 -> lst:list nat
+                   -> Lemma (requires (forall ch. mem ch lst ==> A.mem_key_s ch a /\ A.mem_key_s ch b) /\
+                                            (forall e. A.mem_key_s e a <==> A.mem_key_s e b) /\
+                                     A.unique_keys lst /\ (forall ch. mem ch lst ==> 
+                   (forall e. G.mem_id_s e (A.get_val_s #G.s #G.op ch a) <==> G.mem_id_s e (A.get_val_s #G.s #G.op ch b))) /\
+            (forall ch. mem ch lst ==> (forall e. mem e (A.get_val_s #G.s #G.op ch a) <==> mem e (A.get_val_s #G.s #G.op ch b))) /\
+                              (forall ch. mem ch lst ==> (List.Tot.length (A.get_val_s #G.s #G.op ch a) = List.Tot.length (A.get_val_s #G.s #G.op ch b))) /\
+                         (forall ch. mem ch lst ==> 
+                       (forall e e1. mem e (A.get_val_s #G.s #G.op ch a) /\ mem e1 (A.get_val_s #G.s #G.op ch a) /\ 
+                         G.fst e <> G.fst e1 /\ G.fst e > G.fst e1 /\ G.ord e e1 (A.get_val_s #G.s #G.op ch a)  <==> 
+              mem e (A.get_val_s #G.s #G.op ch b) /\ mem e1 (A.get_val_s #G.s #G.op ch b) /\ G.fst e <> G.fst e1 /\
+                          G.fst e > G.fst e1 /\ G.ord e e1 (A.get_val_s #G.s #G.op ch b))))
+                     (ensures (forall ch. mem ch lst ==> (A.get_val_s #G.s #G.op ch a = A.get_val_s #G.s #G.op ch b)))
+                         (decreases lst)
+#set-options "--z3rlimit 10000000"
+let rec convergence3 a b lst =
+  match lst with
+  |[] -> ()
+  |ch::chs -> G.lem_same (A.get_val_s #G.s #G.op ch a) (A.get_val_s #G.s #G.op ch b);
+            convergence3 a b chs
+
+val convergence_a : tr:ae (A.op G.op)
+                  -> a:A.s G.s
+                  -> b:A.s G.s
+                  -> Lemma (requires (A.sim_a tr a /\ A.sim_a tr b))
+                          (ensures (forall e. A.mem_key_s e a <==> A.mem_key_s e b) /\
+                                      (forall ch. A.mem_key_s ch a /\ A.mem_key_s ch b ==> 
+                               (A.get_val_s #G.s #G.op ch a) = (A.get_val_s #G.s #G.op ch b)))
+
+#set-options "--z3rlimit 100000000"
+let convergence_a tr a b = 
+  A.convergence_a1 tr a b;
+  convergence2 tr a b;
+  lem_length a b (A.get_lst a);
+  convergence3 a b (A.get_lst a)
+
+#set-options "--z3rlimit 10000000" 
+instance _ : mrdt (A.s G.s) (A.op G.op) = {
+  Library.init = A.init_a;
+  Library.sim = A.sim_a;
+  Library.pre_cond_op = A.pre_cond_op_a;
+  Library.app_op = A.app_op_a;
+  Library.prop_oper = prop_oper;
+  Library.pre_cond_merge1 = pre_cond_merge1_a;
+  Library.pre_cond_merge = pre_cond_merge_a;
+  Library.merge1 = merge1_a;
+  Library.merge = merge_a;
+  Library.prop_merge = A.prop_merge_a;
+  Library.convergence = convergence_a;
+}
